README.md
@@ -3,3 +3,4 @@
 * determine whether there is an issue w/ current lax typing on le judgments
 * fill admits in subst lemmas for IExp
 * fill admits (or remove lemmas) for identity operation in Tactics
+* get rule notations compatible with Irule, Arule notations
